coq/ptr_sr.v
@@ -1,0 +1,205 @@
+From mathcomp Require Import ssreflect ssrbool eqtype ssrnat seq.
+From Coq Require Import ssrfun Classical Utf8.
+Require Export AutosubstSsr ARS ptr_step ptr_subst era_sr.
+
+Set Implicit Arguments.
+Unset Strict Implicit.
+Unset Printing Implicit Defensive.
+
+Lemma ptr_sr H1 H2 H H' x y z z' A :
+  H1 ; x ~ y ~ z : A -> wr_heap H ->
+  H1 ∘ H2 => H -> H ; z ~>> H' ; z' ->
+  exists H1' H2' x' y',
+    H1' ; x' ~ y' ~ z' : A /\ wr_heap H' /\
+    pad H2 H2' /\ H1' ∘ H2' => H' /\ x ~>>* x' /\ y ~>>* y'.
+Proof with eauto 7 using pad, era_type, resolve, merge, free, key, dyn_step.
+  move=>{H1 x y z A}[H1 x y z A].
+  move e1:(nil)=>Γ. move e2:(nil)=>Δ er.
+  elim: er H1 H2 H H' z z' e1 e2=>{Γ Δ x y A}.
+  { move=>Γ Δ x s A wf shs dhs H1 H2 H H' z z' e1 e2 rs wr mrg st; subst. inv shs. }
+  { move=>Γ Δ A B m m' s k erm _ H1 H2 H H' z z' e1 e2 rs wr mrg st; subst.
+    inv rs; inv st.
+    have[<-_]:=merge_size mrg.
+    have[wr1 wr2]:=wr_merge_inv mrg wr.
+    destruct s.
+    { exists (Lam0 Box m0 U :U H1).
+      exists (Lam0 Box m0 U :U H2).
+      exists (Lam0 A m U).
+      exists (Lam0 Box m' U).
+      repeat split...
+      { econstructor...
+        constructor...
+        apply: resolve_wkU... }
+      { constructor...
+        have//=nfm':=nf_typing erm.
+        have//:=resolve_wr_nfi H8 wr1 nfm'. } }
+    { exists (Lam0 Box m0 L :L H1).
+      exists (_: H2).
+      exists (Lam0 A m L).
+      exists (Lam0 Box m' L).
+      repeat split...
+      { econstructor...
+        constructor...
+        apply: resolve_wkN... }
+      { constructor...
+        have//=nfm':=nf_typing erm.
+        have//:=resolve_wr_nfi H8 wr1 nfm'. } } }
+  { move=>Γ Δ A B m m' s t k erm _ H1 H2 H H' z z' e1 e2 rs wr mrg st; subst.
+    inv rs; inv st.
+    have[<-_]:=merge_size mrg.
+    have[wr1 wr2]:=wr_merge_inv mrg wr.
+    destruct s.
+    { exists (Lam1 Box m0 U :U H1).
+      exists (Lam1 Box m0 U :U H2).
+      exists (Lam1 A m U).
+      exists (Lam1 Box m' U).
+      repeat split...
+      { econstructor...
+        constructor...
+        apply: resolve_wkU... }
+      { constructor...
+        have//=nfm':=nf_typing erm.
+        have//:=resolve_wr_nfi H8 wr1 nfm'. } }
+    { exists (Lam1 Box m0 L :L H1).
+      exists (_: H2).
+      exists (Lam1 A m L).
+      exists (Lam1 Box m' L).
+      repeat split...
+      { econstructor...
+        constructor...
+        apply: resolve_wkN... }
+      { constructor...
+        have//=nfm':=nf_typing erm.
+        have//:=resolve_wr_nfi H8 wr1 nfm'. } } }
+  { move=>Γ Δ A B m m' n s erm ihm tyn H1 H2 H H' z z' e1 e2 rs wr mrg st; subst.
+    inv rs; inv st.
+    { have[H1'[H2'[x'[y'[wrx[wr'[pd[mrg'[rd1 rd2]]]]]]]]]:=ihm _ _ _ _ _ _ erefl erefl H6 wr mrg H9.
+      inv wrx.
+      exists H1'. exists H2'. exists (App x' n). exists (App y' Box).
+      repeat split...
+      apply: (star_hom (App^~ n)) rd1=>x y.
+      apply: dyn_step_appL.
+      apply: (star_hom (App^~ Box)) rd2=>x y.
+      apply: dyn_step_appL. }
+    { inv H9. }
+    { have[H1'[mrg' rs]]:=resolve_free H9 H6 mrg. inv rs.
+      have[A0[n0 e]]:=era_lam0_form erm. subst.
+      exists H1'. exists H2. exists (n0.[n/]). exists (m'0.[Box/]).
+      repeat split...
+      { have ern0:=era_lam0_inv erm.
+        apply: era_esubst0... }
+      { have ern:=era_lam0_inv erm.
+        have wr':=free_wr H9 wr.
+        have[wr1 wr2]:=wr_merge_inv mrg' wr'.
+        have[Hx[k mrgx]]:=split_self H1'.
+        have[_ wrx]:=wr_merge_inv mrgx wr1.
+        apply: resolve_subst...
+        constructor.
+        constructor... }
+      { apply: free_wr... }
+      { apply: star1... }
+      { apply: star1... } }
+    { have[wr1 wr2]:=wr_merge_inv mrg wr.
+      have[wr3 wr4]:=wr_merge_inv H7 wr1.
+      have//:=resolve_wr_box wr4 H11. }
+    { have[wr1 wr2]:=wr_merge_inv mrg wr.
+      have[wr3 wr4]:=wr_merge_inv H7 wr1.
+      have//:=resolve_wr_box wr4 H11. }
+    { have[wr1 wr2]:=wr_merge_inv mrg wr.
+      have[wr3 wr4]:=wr_merge_inv H7 wr1.
+      have//:=resolve_wr_box wr4 H11. }
+    { have[wr1 wr2]:=wr_merge_inv mrg wr.
+      have[wr3 wr4]:=wr_merge_inv H7 wr1.
+      have//:=resolve_wr_box wr4 H11. } }
+  { move=>Γ Δ1 Δ2 Δ A B m m' n n' s mrg1 erm ihm ern ihn H1 H2 H H' z z' e1 e2 rs wr mrg2 st; subst.
+    inv mrg1. inv rs; inv st.
+    { have//:=era_box_form ern. }
+    { have//:=era_box_form ern. }
+    { have//:=era_box_form ern. }
+    { have[wr1 wr2]:=wr_merge_inv mrg2 wr.
+      have[H4[mrg3 mrg4]]:=merge_splitR mrg2 H7.
+      have[H1'[H2'[x'[y'[wrx[wr'[pd[mrg5[rd1 rd2]]]]]]]]]:=
+        ihm _ _ _ _ _ _ erefl erefl H10 wr (merge_sym mrg4) H13.
+      have[H1p[H2p[pd1[pd2 mrp]]]]:=pad_merge pd mrg3.
+      have[Hx[mrp1 mrp2]]:=merge_splitL (merge_sym mrg5) mrp.
+      inv wrx.
+      exists Hx. exists H2p. exists (App x' n). exists (App y' n').
+      repeat split...
+      { econstructor.
+        apply: merge_sym...
+        apply: H8.
+        apply: resolve_pad... }
+      { apply: (star_hom (App^~ n)) rd1=>x y.
+        apply: dyn_step_appL. }
+      { apply: (star_hom (App^~ n')) rd2=>x y.
+        apply: dyn_step_appL. } }
+    { have[H4[mrg3 mrg4]]:=merge_splitL mrg2 H7.
+      have[H1'[H2'[x'[y'[wrx[wr'[pd[mrg5[rd1 rd2]]]]]]]]]:=
+        ihn _ _ _ _ _ _ erefl erefl H11 wr (merge_sym mrg4) H13.
+      have[H1p[H2p[pd1[pd2 mrp]]]]:=pad_merge pd mrg3.
+      have[Hx[mrp1 mrp2]]:=merge_splitL (merge_sym mrg5) mrp.
+      inv wrx.
+      exists Hx. exists H2p. exists (App m x'). exists (App m' y').
+      repeat split...
+      { have[t tyP]:=dyn_valid (era_dyn_type erm).
+        have[r[tyB/sort_inj e]]:=sta_pi1_inv tyP. subst.
+        have tyn:=dyn_sta_type (era_dyn_type ern).
+        have//=tyBn:=sta_subst tyB tyn.
+        apply: era_conv.
+        apply: sta_conv_beta.
+        apply: conv_sym.
+        apply: star_conv.
+        apply: dyn_sta_red...
+        econstructor...
+        apply: tyBn. }
+      { econstructor...
+        apply: resolve_pad... }
+      { apply: (star_hom (App m)) rd1=>x y.
+        apply: dyn_step_appR. }
+      { apply: (star_hom (App m')) rd2=>x y.
+        apply: dyn_step_appR. } }
+    { have[Hx[mrg3 mrg4]]:=merge_splitR mrg2 H7.
+      have[Hy[mrg5 rs]]:=resolve_free H13 H10 (merge_sym mrg4). inv rs.
+      have[A0[n1 e]]:=era_lam0_form erm. subst.
+      exfalso. apply: sta_lam0_pi1_false... }
+    { have[H4[mrg3 mrg4]]:=merge_splitR mrg2 H7.
+      have[H5[mrg rs]]:=resolve_free H13 H10 (merge_sym mrg4). inv rs.
+      have[Hx[mrg5 mrg6]]:=merge_splitL (merge_sym mrg) mrg3.
+      have[A0[n0 e]]:=era_lam1_form erm. subst.
+      have[r ern0]:=era_lam1_inv erm.
+      have wr':=free_wr H13 wr.
+      have[wr1 wr2]:=wr_merge_inv mrg wr'.
+      have[wr3 wr4]:=wr_merge_inv mrg3 wr2.
+      have[H3'[k mrg']]:=split_self H3.
+      have[_ wr3']:=wr_merge_inv mrg' wr3.
+      have vl':=wr_resolve_ptr wr3 H11.
+      have vl:=era_dyn_val ern vl'.
+      exists Hx. exists H2. exists n0.[n/]. exists m'0.[n'/].
+      repeat split...
+      { apply: era_subst1.
+        apply: key_nil.
+        apply: merge_nil.
+        apply: ern0.
+        apply: ern. }
+      { have wf:=dyn_type_wf (era_dyn_type ern0). inv wf.
+        have k1:=resolution (Ptr_well_resolved ern H11) H17 vl' wr3.
+        destruct r.
+        { apply: resolve_subst.
+          apply: ern0.
+          apply: merge_sym...
+          apply: H16.
+          apply: wr1.
+          apply: agree_resolve_wkU.
+          apply: merge_sym...
+          all: eauto.
+          constructor... }
+        { apply: resolve_subst.
+          apply: ern0.
+          apply: merge_sym...
+          all: eauto.
+          apply: agree_resolve_wkL.
+          apply: merge_sym...
+          all: eauto.
+          constructor... } }
+      { apply: star1. apply: dyn_step_beta1... }
+      { apply: star1. apply: dyn_step_beta1... } } }
