coq/sta_step.v
@@ -6,7 +6,7 @@ Set Implicit Arguments.
 Unset Strict Implicit.
 Unset Printing Implicit Defensive.
 
-Reserved Notation "m ~> n" (at level 30).
+Reserved Notation "m ~> n" (at level 50).
 Inductive sta_step : term -> term -> Prop :=
 | sta_step_pi0L A A' B s :
   A ~> A' ->
